theories/NormalForms.v
@@ -3,6 +3,66 @@ From Coq Require Import ssrbool.
 From LogRel.AutoSubst Require Import core unscoped Ast Extra.
 From LogRel Require Import Utils BasicAst Context.
 
+(** Deep normal forms *)
+
+Definition isLambda (t : term) := match t with
+| tLambda _ _ => true
+| _ => false
+end.
+
+Definition isNatConstructor (t : term) := match t with
+| tZero | tSucc _ => true
+| _ => false
+end.
+
+Definition isPairConstructor (t : term) := match t with
+| tPair _ _ _ _ => true
+| _ => false
+end.
+
+Definition isEmptyConstructor (t : term) := false.
+
+Definition isIdConstructor (t : term) := match t with
+| tRefl _ _ => true
+| _ => false
+end.
+
+Unset Elimination Schemes.
+
+Inductive dnf : term -> Set :=
+  | dnf_tSort {s} : dnf (tSort s)
+  | dnf_tProd {A B} : dnf A -> dnf B -> dnf (tProd A B)
+  | dnf_tLambda {A t} : dnf A -> dnf t -> dnf (tLambda A t)
+  | dnf_tNat : dnf tNat
+  | dnf_tZero : dnf tZero
+  | dnf_tSucc {n} : dnf n -> dnf (tSucc n)
+  | dnf_tEmpty : dnf tEmpty
+  | dnf_tSig {A B} : dnf A -> dnf B -> dnf (tSig A B)
+  | dnf_tPair {A B a b} : dnf A -> dnf B -> dnf a -> dnf b -> dnf (tPair A B a b)
+  | dnf_tId {A x y} : dnf A -> dnf x -> dnf y -> dnf (tId A x y)
+  | dnf_tRefl {A x} : dnf A -> dnf x -> dnf (tRefl A x)
+  | dnf_dne {n} : dne n -> dnf n
+with dne : term -> Set :=
+  | dne_tRel {v} : dne (tRel v)
+  | dne_tApp {n t} : dne n -> dnf t -> dne (tApp n t)
+  | dne_tNatElim {P hz hs n} : dnf P -> dnf hz -> dnf hs -> dne n -> dne (tNatElim P hz hs n)
+  | dne_tEmptyElim {P n} : dnf P -> dne n -> dne (tEmptyElim P n)
+  | dne_tFst {n} : dne n -> dne (tFst n)
+  | dne_tSnd {n} : dne n -> dne (tSnd n)
+  | dne_tIdElim {A x P hr y e} : dnf A -> dnf x -> dnf P -> dnf hr -> dnf y -> dne e -> dne (tIdElim A x P hr y e)
+.
+
+Set Elimination Schemes.
+
+Scheme
+  Induction for dnf Sort Type with
+  Induction for dne Sort Type.
+
+Definition dnf_dne_rect P Q p1 p2 p3 p4 p5 p6 p7 p8 p9 p10 p11 p12 p13 p14 p15 p16 p17 p18 p19 :=
+  pair
+    (dnf_rect P Q p1 p2 p3 p4 p5 p6 p7 p8 p9 p10 p11 p12 p13 p14 p15 p16 p17 p18 p19)
+    (dne_rect P Q p1 p2 p3 p4 p5 p6 p7 p8 p9 p10 p11 p12 p13 p14 p15 p16 p17 p18 p19).
+
 (** ** Weak-head normal forms and neutrals. *)
 
 Inductive whnf : term -> Type :=
@@ -35,6 +95,26 @@ Ltac inv_whne :=
     try solve [inversion H] ; block H
   end; unblock.
 
+Lemma dnf_dne_whnf_whne : (forall v, dnf v -> whnf v) × (forall n, dne n -> whne n).
+Proof.
+apply dnf_dne_rect; intros; now constructor.
+Qed.
+
+Lemma dnf_whnf : forall v, dnf v -> whnf v.
+Proof.
+intros; now apply dnf_dne_whnf_whne.
+Qed.
+
+Lemma dne_whne : forall v, dne v -> whne v.
+Proof.
+intros; now apply dnf_dne_whnf_whne.
+Qed.
+
+Lemma dne_dnf_whne : forall v, dnf v -> whne v -> dne v.
+Proof.
+intros v [] H; inversion H; subst; tea.
+Qed.
+
 Lemma neSort s : whne (tSort s) -> False.
 Proof.
   inversion 1.
@@ -49,6 +129,63 @@ Lemma neLambda A t : whne (tLambda A t) -> False.
 Proof.
   inversion 1.
 Qed.
+
+Section RenDnf.
+
+Lemma dnf_dne_ren : (forall t, dnf t -> forall ρ, dnf t⟨ρ⟩) × (forall t, dne t -> forall ρ, dne t⟨ρ⟩).
+Proof.
+apply dnf_dne_rect; cbn; intros; try now econstructor.
+Qed.
+
+Local Ltac inv_dne := try match goal with H : dne _ |- _ => inversion H; subst end.
+
+Lemma dnf_dne_ren_rev : forall t ρ, (dnf t⟨ρ⟩ -> dnf t) × (whne t⟨ρ⟩ -> whne t).
+Proof.
+induction t; intros ρ; split; cbn in *; intros; inv_whne.
+all: repeat match goal with H : forall ρ, (_ × _) |- _ =>
+  pose proof (fun ρ => fst (H ρ));
+  pose proof (fun ρ => snd (H ρ));
+  clear H
+end.
+all: repeat match goal with H : dnf ?t |- _ => is_var t; inversion H; subst; clear H end.
+all: try now (constructor; match goal with H : whne _ |- _ => inversion H end; subst).
+all: try now (match goal with H : dnf ?t |- _ => inversion H; subst; clear H end; inv_dne; constructor).
+all: try now (
+  match goal with H : dnf ?t |- _ => inversion H; subst; clear H end;
+  match goal with H : dne ?t |- _ => inversion H; subst; clear H end;
+  do 2 constructor; eauto; apply dne_dnf_whne; eauto using dnf_dne, dne_whne).
+Qed.
+
+Lemma dnf_ren_rev : forall t ρ, dnf t⟨ρ⟩ -> dnf t.
+Proof.
+intros; now eapply dnf_dne_ren_rev.
+Qed.
+
+Lemma dne_ren_rev : forall t ρ, dne t⟨ρ⟩ -> dne t.
+Proof.
+intros.
+eapply dne_dnf_whne.
++ eapply dnf_dne_ren_rev; now constructor.
++ apply dnf_dne_whnf_whne in H.
+  now apply dnf_dne_ren_rev in H.
+Qed.
+
+Lemma whne_ren_rev : forall t ρ, whne t⟨ρ⟩ -> whne t.
+Proof.
+intros; now eapply dnf_dne_ren_rev.
+Qed.
+
+Lemma dne_ren ρ (t : term) : dne t -> dne t⟨ρ⟩.
+Proof.
+intros; now apply dnf_dne_ren.
+Qed.
+
+Lemma dnf_ren ρ (t : term) : dnf t -> dnf t⟨ρ⟩.
+Proof.
+intros; now apply dnf_dne_ren.
+Qed.
+
+End RenDnf.
 
 #[global] Hint Resolve neSort nePi neLambda : gen_typing.
 
