theories/UntypedReduction.v
@@ -1,5 +1,5 @@
 (** * LogRel.UntypedReduction: untyped reduction, used to define algorithmic typing.*)
-From Coq Require Import CRelationClasses.
+From Coq Require Import CRelationClasses ssrbool.
 From LogRel.AutoSubst Require Import core unscoped Ast Extra.
 From LogRel Require Import Utils BasicAst Notations Context NormalForms Weakening.
 
@@ -7,13 +7,15 @@ From LogRel Require Import Utils BasicAst Notations Context NormalForms Weakenin
 
 (** *** One-step reduction. *)
 
-Inductive OneRedAlg : term -> term -> Type :=
+Inductive OneRedAlg {deep : bool} : term -> term -> Type :=
 | BRed {A a t} :
     [ tApp (tLambda A t) a ⤳ t[a..] ]
 | appSubst {t u a} :
+    negb (isLambda t) ->
     [ t ⤳ u ] ->
     [ tApp t a ⤳ tApp u a ]
 | natElimSubst {P hz hs n n'} :
+    negb (isNatConstructor n) ->
     [ n ⤳ n' ] ->
     [ tNatElim P hz hs n ⤳ tNatElim P hz hs n' ]
 | natElimZero {P hz hs} :
@@ -21,14 +23,17 @@ Inductive OneRedAlg : term -> term -> Type :=
 | natElimSucc {P hz hs n} :
     [ tNatElim P hz hs (tSucc n) ⤳ tApp (tApp hs n) (tNatElim P hz hs n) ]
 | emptyElimSubst {P e e'} :
+    negb (isEmptyConstructor e) ->
     [e ⤳ e'] ->
     [tEmptyElim P e ⤳ tEmptyElim P e']        
 | fstSubst {p p'} :
+    negb (isPairConstructor p) ->
     [ p ⤳ p'] ->
     [ tFst p ⤳ tFst p']
 | fstPair {A B a b} :
     [ tFst (tPair A B a b) ⤳ a ]
 | sndSubst {p p'} :
+    negb (isPairConstructor p) ->
     [ p ⤳ p'] ->
     [ tSnd p ⤳ tSnd p']
 | sndPair {A B a b} :
@@ -36,25 +41,96 @@ Inductive OneRedAlg : term -> term -> Type :=
 | idElimRefl {A x P hr y A' z} :
   [ tIdElim A x P hr y (tRefl A' z) ⤳ hr ]
 | idElimSubst {A x P hr y e e'} :
+  negb (isIdConstructor e) ->
   [e ⤳ e'] ->
   [ tIdElim A x P hr y e ⤳ tIdElim A x P hr y e' ]
 
+(* Hereditary normal forms *)
+
+| prodDom {A A' B} : deep ->
+  [ A ⤳ A' ] -> [ tProd A B ⤳ tProd A' B ]
+| prodCod {A B B'} : deep ->
+  dnf A -> [ B ⤳ B' ] -> [ tProd A B ⤳ tProd A B' ]
+| lamDom {A A' t} : deep ->
+  [ A ⤳ A' ] -> [ tLambda A t ⤳ tLambda A' t ]
+| lamBody {A t t'} : deep ->
+  dnf A -> [ t ⤳ t' ] -> [ tLambda A t ⤳ tLambda A t' ]
+| appSubstNe {t u u'} : deep ->
+  dne t -> [ u ⤳ u' ] -> [ tApp t u ⤳ tApp t u' ]
+| succArg {t t'} : deep ->
+  [ t ⤳ t' ] -> [ tSucc t ⤳ tSucc t' ]
+| natElimPred {P P' hz hs n} : deep ->
+  dne n -> [ P ⤳ P' ] -> [ tNatElim P hz hs n ⤳ tNatElim P' hz hs n ]
+| natElimBranchZero {P hz hz' hs n} : deep ->
+  dne n -> dnf P -> [ hz ⤳ hz' ] -> [ tNatElim P hz hs n ⤳ tNatElim P hz' hs n ]
+| natElimBranchSucc {P hz hs hs' n} : deep ->
+  dne n -> dnf P -> dnf hz -> [ hs ⤳ hs' ] -> [ tNatElim P hz hs n ⤳ tNatElim P hz hs' n ]
+| emptyElimPred {P P' n} : deep ->
+  dne n -> [ P ⤳ P' ] -> [ tEmptyElim P n ⤳ tEmptyElim P' n ]
+| sigDom {A A' B} : deep ->
+  [ A ⤳ A' ] -> [ tSig A B ⤳ tSig A' B ]
+| sigCod {A B B'} : deep ->
+  dnf A ->
+  [ B ⤳ B' ] -> [ tSig A B ⤳ tSig A B' ]
+| pairDom {A A' B a b} : deep ->
+  [ A ⤳ A' ] -> [ tPair A B a b ⤳ tPair A' B a b ]
+| pairCod {A B B' a b} : deep ->
+  dnf A ->
+  [ B ⤳ B' ] -> [ tPair A B a b ⤳ tPair A B' a b ]
+| pairFst {A B a a' b} : deep ->
+  dnf A -> dnf B ->
+  [ a ⤳ a' ] -> [ tPair A B a b ⤳ tPair A B a' b ]
+| pairSnd {A B a b b'} : deep ->
+  dnf A -> dnf B -> dnf a ->
+  [ b ⤳ b' ] -> [ tPair A B a b ⤳ tPair A B a b' ]
+| idDom {A A' t u} : deep ->
+  [ A ⤳ A' ] -> [ tId A t u ⤳ tId A' t u ]
+| idLHS {A t t' u} : deep ->
+  dnf A -> [ t ⤳ t' ] -> [ tId A t u ⤳ tId A t' u ]
+| idRHS {A t u u'} : deep ->
+  dnf A -> dnf t -> [ u ⤳ u' ] -> [ tId A t u ⤳ tId A t u' ]
+| reflDom {A A' t} : deep ->
+  [ A ⤳ A' ] -> [ tRefl A t ⤳ tRefl A' t ]
+| reflArg {A t t'} : deep ->
+  dnf A -> [ t ⤳ t' ] -> [ tRefl A t ⤳ tRefl A t' ]
+| idElimDom {A A' x P hr y e} : deep ->
+  dne e ->
+  [ A ⤳ A' ] -> [ tIdElim A x P hr y e ⤳ tIdElim A' x P hr y e ]
+| idElimLHS {A x x' P hr y e} : deep ->
+  dne e -> dnf A ->
+  [ x ⤳ x' ] -> [ tIdElim A x P hr y e ⤳ tIdElim A x' P hr y e ]
+| idElimPred {A x P P' hr y e} : deep ->
+  dne e -> dnf A -> dnf x ->
+  [ P ⤳ P' ] -> [ tIdElim A x P hr y e ⤳ tIdElim A x P' hr y e ]
+| idElimBranchRefl {A x P hr hr' y e} : deep ->
+  dne e -> dnf A -> dnf x -> dnf P ->
+  [ hr ⤳ hr' ] -> [ tIdElim A x P hr y e ⤳ tIdElim A x P hr' y e ]
+| idElimRHS {A x P hr y y' e} : deep ->
+  dne e -> dnf A -> dnf x -> dnf P -> dnf hr ->
+  [ y ⤳ y' ] -> [ tIdElim A x P hr y e ⤳ tIdElim A x P hr y' e ]
+
 where "[ t ⤳ t' ]" := (OneRedAlg t t') : typing_scope.
+
+Notation "[ t ⤳ t' ]" := (OneRedAlg (deep := false) t t') : typing_scope.
+Notation "[ t ⇶ t' ]" := (OneRedAlg (deep := true) t t') : typing_scope.
 
 (* Keep in sync with OneRedTermDecl! *)
 
 (** *** Multi-step reduction *)
 
-Inductive RedClosureAlg : term -> term -> Type :=
+Inductive RedClosureAlg {deep : bool} : term -> term -> Type :=
   | redIdAlg {t} :
     [ t ⤳* t ]
   | redSuccAlg {t t' u} :
-    [ t ⤳ t'] ->
+    @OneRedAlg deep t t' ->
     [ t' ⤳* u ] ->
     [ t ⤳* u ]
   where "[ t ⤳* t' ]" := (RedClosureAlg t t') : typing_scope.
 
-#[export] Instance RedAlgTrans : PreOrder RedClosureAlg.
+Notation "[ t ⤳* t' ]" := (RedClosureAlg (deep := false) t t') : typing_scope.
+Notation "[ t ⇶* t' ]" := (RedClosureAlg (deep := true) t t') : typing_scope.
+
+#[export] Instance RedAlgTrans {deep} : PreOrder (@RedClosureAlg deep).
   Proof.
     split.
     - now econstructor.
@@ -66,7 +142,52 @@ Inductive RedClosureAlg : term -> term -> Type :=
 
 (** ** Properties *)
 
+(** Inclusions *)
+
+Lemma dred_ored : forall t t', [ t ⤳ t' ] -> [ t ⇶ t' ].
+Proof.
+intros t t'; induction 1; now econstructor.
+Qed.
+
+Lemma dred_red : forall t t', [ t ⤳* t' ] -> [ t ⇶* t' ].
+Proof.
+induction 1; econstructor; tea.
+now apply dred_ored.
+Qed.
+
 (** *** Weak-head normal forms do not reduce *)
+
+Lemma dnf_dne_nogred :
+  (forall t, dnf t -> forall deep u, OneRedAlg (deep := deep) t u -> False) × (forall n, dne n -> forall deep u, OneRedAlg (deep := deep) n u -> False).
+Proof.
+apply dnf_dne_rect; intros.
+all: match goal with
+| H : OneRedAlg _ _ |- _ => inversion H; subst
+end; try now intuition.
+all: match goal with H : dne _ |- _ => solve [inversion H] end.
+Qed.
+
+Lemma dnf_dne_nored :
+  (forall t, dnf t -> forall u, [t ⇶ u] -> False) × (forall n, dne n -> forall u, [n ⇶ u] -> False).
+Proof.
+apply dnf_dne_rect; intros.
+all: match goal with
+| H : [_ ⇶ _] |- _ => inversion H; subst
+end; try now intuition.
+all: match goal with H : dne _ |- _ => solve [inversion H] end.
+Qed.
+
+Lemma dnf_nored : forall t u, dnf t -> [t ⇶ u] -> False.
+Proof.
+intros t u H Hr.
+destruct dnf_dne_nored as [f _]; now eapply f.
+Qed.
+
+Lemma dne_nored : forall t u, dne t -> [t ⇶ u] -> False.
+Proof.
+intros t u H Hr.
+destruct dnf_dne_nored as [_ f]; now eapply f.
+Qed.
 
 Ltac inv_whne :=
   match goal with [ H : whne _ |- _ ] => inversion H end.
@@ -74,67 +195,84 @@ Ltac inv_whne :=
 Lemma whne_nored n u :
   whne n -> [n ⤳ u] -> False.
 Proof.
+  remember false as deep eqn: Hd.
   intros ne red.
-  induction red in ne |- *.
-  all: inversion ne ; subst ; clear ne.
-  2: auto.
-  all: now inv_whne.
+  revert Hd; induction red; intros Hd.
+  all: inversion ne ; subst ; clear ne; auto.
+  all: inv_whne.
 Qed.
 
 Lemma whnf_nored n u :
   whnf n -> [n ⤳ u] -> False.
 Proof.
+  remember false as deep eqn: Hd.
   intros nf red.
-  induction red in nf |- *.
-  2,3,6,7,9,12: inversion nf; subst; inv_whne; subst; apply IHred; now constructor.
-  all: inversion nf; subst; inv_whne; subst; try now inv_whne.
+  revert Hd; induction red; intros Hd.
+  all: inversion nf; subst; auto.
+  - inversion H ; subst.
+    now eapply neLambda.
+  - inversion H ; subst.
+    eapply IHred; [|trivial].
+    now constructor.
+  - inversion H ; subst.
+    eapply IHred; [|trivial].
+    now constructor.
+  - inversion H ; subst.
+    inv_whne.
+  - inversion H ; subst.
+    inv_whne.
+  - inversion H; subst.
+    eapply IHred; [|trivial].
+    now constructor.
+  - inversion H; subst.
+    eapply IHred; [|trivial].
+    now constructor.
+  - inversion H; subst.
+    inversion H1; subst.
+  - inversion H; subst.
+    eapply IHred; [|trivial].
+    now constructor.
+  - inversion H; subst.
+    inversion H1; subst.
+  - inversion H; subst.
+    inversion H1.
+  - inversion H; subst.
+    eapply IHred; [|trivial].
+    now constructor.
 Qed.
 
 (** *** Determinism of reduction *)
+
+Lemma gred_det {deep t u v} :
+  OneRedAlg (deep := deep) t u ->
+  OneRedAlg (deep := deep) t v ->
+  u = v.
+Proof.
+intros Hu Hv; revert v Hv; induction Hu; intros v Hv; inversion Hv; subst; simpl in *.
+all: match goal with
+| _ => reflexivity
+| H : is_true false |- _ => elim notF; exact H
+| H : dne _ |- _ => now inversion H
+| H : dne _ |- _ => now eapply dnf_dne_nogred in H
+| H : dnf _ |- _ => now eapply dnf_dne_nogred in H
+| H : [ ?t ⇶ ?u ] |- _ => now inversion H
+| _ => now f_equal
+| _ => idtac
+end.
+Qed.
+
+Lemma dred_det {t u v} :
+  [t ⇶ u] -> [t ⇶ v] ->
+  u = v.
+Proof.
+apply gred_det.
+Qed.
 
 Lemma ored_det {t u v} :
   [t ⤳ u] -> [t ⤳ v] ->
   u = v.
 Proof.
-  intros red red'.
-  induction red in v, red' |- *.
-  - inversion red' ; subst ; clear red'.
-    + reflexivity.
-    + exfalso.
-      eapply whnf_nored.
-      2: eassumption.
-      now econstructor.
-  - inversion red' ; subst ; clear red'.
-    + exfalso.
-      eapply whnf_nored.
-      2: eassumption.
-      now econstructor.
-    + f_equal.
-      eauto.
-  - inversion red'; subst.
-    2,3: exfalso; eapply whnf_nored; tea; constructor.
-    f_equal; eauto.
-  - inversion red'; try reflexivity; subst.
-    exfalso; eapply whnf_nored; tea; constructor.
-  - inversion red'; try reflexivity; subst.
-    exfalso; eapply whnf_nored; tea; constructor.
-  - inversion red'; subst.
-    f_equal; eauto.
-  - inversion red'; subst; clear red'.
-    1: f_equal; now eapply IHred.
-    exfalso; eapply whnf_nored; tea; constructor.
-  - inversion red'; subst; try reflexivity.
-    exfalso; eapply whnf_nored; tea; constructor.
-  - inversion red'; subst; clear red'.
-    1: f_equal; now eapply IHred.
-    exfalso; eapply whnf_nored; tea; constructor.
-  - inversion red'; subst; try reflexivity.
-    exfalso; eapply whnf_nored; tea; constructor.
-  - inversion red'; subst; try reflexivity.
-    exfalso; eapply whnf_nored;tea; constructor.
-  - inversion red'; subst.
-    2: f_equal; eauto.
-    exfalso; eapply whnf_nored;tea; constructor.
+intros; eapply dred_det; now eapply dred_ored.
 Qed.
 
 Lemma red_whne t u : [t ⤳* u] -> whne t -> t = u.
@@ -145,12 +283,33 @@ Proof.
   eauto using whne_nored.
 Qed.
 
+Lemma dred_whne : forall t u, [t ⇶ u] -> whne t -> whne u.
+Proof.
+intros t u Hr Ht; revert u Hr.
+induction Ht; intros u Hr; inversion Hr; subst; first [constructor; now eauto|now inv_whne|idtac].
+Qed.
+
+Lemma dredalg_whne : forall t u, [t ⇶* u] -> whne t -> whne u.
+Proof.
+intros * H Hne.
+induction H; [tea|].
+now eauto using dred_whne.
+Qed.
+
 Lemma red_whnf t u : [t ⤳* u] -> whnf t -> t = u.
 Proof.
   intros [] ?.
   1: reflexivity.
   exfalso.
   eauto using whnf_nored.
+Qed.
+
+Lemma dred_dnf t u : [t ⇶* u] -> dnf t -> t = u.
+Proof.
+  intros [] ?.
+  1: reflexivity.
+  exfalso.
+  eauto using dnf_nored.
 Qed.
 
 Lemma whred_red_det t u u' :
@@ -168,6 +327,21 @@ Proof.
       now eapply IHred.
 Qed.
 
+Lemma dred_red_det t u u' :
+  dnf u ->
+  [t ⇶* u] -> [t ⇶* u'] ->
+  [u' ⇶* u].
+Proof.
+  intros whnf red red'.
+  induction red in whnf, u', red' |- *.
+  - inversion red'; subst; [reflexivity|].
+    now eelim dnf_nored.
+  - destruct red' as [|? ? ? o'].
+    + now econstructor.
+    + eapply IHred; [tea|].
+      now unshelve epose proof (dred_det o o') as <-.
+Qed.
+
 Corollary whred_det t u u' :
   whnf u -> whnf u' ->
   [t ⤳* u] -> [t ⤳* u'] ->
@@ -178,28 +352,230 @@ Proof.
   now eapply whred_red_det.
 Qed.
 
+Corollary dredalg_det t u u' :
+  dnf u -> dnf u' ->
+  [t ⇶* u] -> [t ⇶* u'] ->
+  u = u'.
+Proof.
+  intros.
+  eapply dred_dnf ; tea.
+  now eapply dred_red_det.
+Qed.
+
+(** Helpers *)
+
+Lemma oredalg_appSubst t t' u :
+  [ t ⤳ t' ] -> [ tApp t u ⤳ tApp t' u ].
+Proof.
+intros; constructor; [|eassumption].
+assert (Hw : ~ whnf t) by (intro; now eelim whnf_nored).
+destruct t; first [now (elim Hw; constructor)|constructor].
+Qed.
+
+Lemma oredalg_natElimSubst {P hz hs n n'} :
+  [ n ⤳ n' ] ->
+  [ tNatElim P hz hs n ⤳ tNatElim P hz hs n' ].
+Proof.
+intros; constructor; [|eassumption].
+assert (Hw : ~ whnf n) by (intro; now eelim whnf_nored).
+destruct n; first [now (elim Hw; constructor)|constructor].
+Qed.
+
 (** *** Stability by weakening *)
+
+Lemma gredalg_wk {deep} (ρ : nat -> nat) (t u : term) : OneRedAlg (deep := deep) t u ->  OneRedAlg (deep := deep)  t⟨ρ⟩ u⟨ρ⟩.
+Proof.
+intros Hred; induction Hred in ρ |- *; cbn.
+all: try now (econstructor; intuition).
+all: try now (econstructor; try apply dnf_ren; try apply dne_ren; intuition).
++ replace (t[a..]⟨ρ⟩) with (t⟨upRen_term_term ρ⟩)[a⟨ρ⟩..] by now bsimpl.
+  now constructor.
++ constructor; [|now intuition].
+  destruct t; first [constructor|now elim notF].
++ constructor; [|now intuition].
+  destruct n; first [constructor|now elim notF].
++ constructor; [|now intuition].
+  destruct p; first [constructor|now elim notF].
++ constructor; [|now intuition].
+  destruct p; first [constructor|now elim notF].
++ constructor; [|now intuition].
+  destruct e; first [constructor|now elim notF].
+Qed.
 
 Lemma oredalg_wk (ρ : nat -> nat) (t u : term) :
 [t ⤳ u] ->
 [t⟨ρ⟩ ⤳ u⟨ρ⟩].
 Proof.
-  intros Hred.
-  induction Hred in ρ |- *.
-  2-5,6-12: cbn; asimpl; now econstructor.
-  - cbn ; asimpl.
-    evar (t' : term).
-    replace (subst_term _ t) with t'.
-    all: subst t'.
-    1: econstructor.
-    now asimpl.
+apply gredalg_wk.
+Qed.
+
+Lemma gcredalg_wk {deep} (ρ : nat -> nat) (t u : term) : RedClosureAlg (deep := deep) t u -> RedClosureAlg (deep := deep)  t⟨ρ⟩ u⟨ρ⟩.
+Proof.
+induction 1; econstructor; eauto using gredalg_wk.
 Qed.
 
 Lemma credalg_wk (ρ : nat -> nat) (t u : term) :
 [t ⤳* u] ->
 [t⟨ρ⟩ ⤳* u⟨ρ⟩].
 Proof.
-  induction 1 ; econstructor ; eauto using oredalg_wk.
+apply gcredalg_wk.
+Qed.
+
+(** Invertibility *)
+
+Lemma redalg_app_inv : forall n n' t t', whne n -> [tApp n t ⇶* tApp n' t'] -> [n ⇶* n'].
+Proof.
+intros n n' t t' Hn Hr.
+remember (tApp n t) as a eqn:Ha.
+remember (tApp n' t') as a' eqn:Ha'.
+revert n n' t t' Ha Ha' Hn.
+induction Hr; intros; subst.
++ injection Ha'; intros; subst; reflexivity.
++ inversion o; subst; [inversion Hn| |].
+  - econstructor; [tea|eapply IHHr]; try reflexivity.
+    eapply dredalg_whne; tea.
+    econstructor; [tea|reflexivity].
+  - eapply IHHr; tea; reflexivity.
+Qed.
+
+Lemma redalg_fst_inv : forall n n', whne n -> [tFst n ⇶* tFst n'] -> [n ⇶* n'].
+Proof.
+intros n n' Hn Hr.
+remember (tFst n) as a eqn:Ha.
+remember (tFst n') as a' eqn:Ha'.
+revert n n' Ha Ha' Hn.
+induction Hr; intros; subst.
++ injection Ha'; intros; subst; reflexivity.
++ inversion o; subst.
+  - econstructor; [tea|eapply IHHr]; try reflexivity.
+    eapply dredalg_whne; tea.
+    econstructor; [tea|reflexivity].
+  - inv_whne.
+Qed.
+
+Lemma dred_ren_inv : forall t u ρ, ren_inj ρ -> [t⟨ρ⟩ ⇶ u⟨ρ⟩] -> [t ⇶ u].
+Proof.
+intros t u ρ Hρ Hr.
+remember t⟨ρ⟩ as t' eqn:Ht.
+remember u⟨ρ⟩ as u' eqn:Hu.
+revert t u ρ Ht Hu Hρ; induction Hr; intros t₀ u₀ ρ Ht Hu Hρ.
+all: repeat match goal with H : _ = ?t⟨?ρ⟩ |- _ =>
+  destruct t; cbn in *; try discriminate; [idtac];
+  try injection H; intros; subst
+end.
+all: repeat (match goal with H : ?t⟨?ρ⟩ = ?u⟨?ρ⟩ |- _ =>
+  apply ren_inj_inv in H; [|eauto using upRen_term_term_inj]; []; subst; clear H
+end).
+all: try now (constructor; eauto using dne_ren_rev, dnf_ren_rev, upRen_term_term_inj).
++ assert (Hrw : forall t u, t⟨upRen_term_term ρ⟩[(u⟨ρ⟩)..] = (t[u..])⟨ρ⟩) by now asimpl.
+  rewrite Hrw in Hu; apply ren_inj_inv in Hu; tea.
+  subst; constructor.
++ assert (forall t, isLambda t -> isLambda t⟨ρ⟩) by now intros [].
+  constructor; eauto using contraNN.
++ assert (forall t, isNatConstructor t -> isNatConstructor t⟨ρ⟩) by now intros [].
+  constructor; eauto using contraNN.
++ assert (forall t, isPairConstructor t -> isPairConstructor t⟨ρ⟩) by now intros [].
+  constructor; eauto using contraNN.
++ assert (forall t, isPairConstructor t -> isPairConstructor t⟨ρ⟩) by now intros [].
+  constructor; eauto using contraNN.
++ assert (forall t, isIdConstructor t -> isIdConstructor t⟨ρ⟩).
+  { intros []; cbn in *; eauto. }
+  constructor; eauto using contraNN.
+Qed.
+
+Ltac unren t := lazymatch t with
+| ?t⟨?ρ⟩ => open_constr:(_ : term)
+| tProd ?t ?u =>
+  let t := unren t in
+  let u := unren u in
+  constr:(tProd t u)
+| tSig ?t ?u =>
+  let t := unren t in
+  let u := unren u in
+  constr:(tSig t u)
+| tApp ?t ?u =>
+  let t := unren t in
+  let u := unren u in
+  constr:(tApp t u)
+| tLambda ?t ?u =>
+  let t := unren t in
+  let u := unren u in
+  constr:(tLambda t u)
+| tFst ?t =>
+  let t := unren t in
+  constr:(tFst t)
+| tSnd ?t =>
+  let t := unren t in
+  constr:(tSnd t)
+| tSucc ?t =>
+  let t := unren t in
+  constr:(tSucc t)
+| tNatElim ?P ?hz ?hs ?t =>
+  let P := unren P in
+  let hz := unren hz in
+  let hs := unren hs in
+  let t := unren t in
+  constr:(tNatElim P hz hs t)
+| tId ?A ?x ?y =>
+  let A := unren A in
+  let x := unren x in
+  let y := unren y in
+  constr:(tId A x y)
+| tRefl ?t ?u =>
+  let t := unren t in
+  let u := unren u in
+  constr:(tRefl t u)
+| tIdElim ?A ?x ?P ?hr ?y ?t =>
+  let A := unren A in
+  let x := unren x in
+  let P := unren P in
+  let hr := unren hr in
+  let y := unren y in
+  let t := unren t in
+  constr:(tIdElim A x P hr y t)
+| tEmptyElim ?P ?t =>
+  let P := unren P in
+  let t := unren t in
+  constr:(tEmptyElim P t)
+| tPair ?A ?B ?a ?b =>
+  let A := unren A in
+  let B := unren B in
+  let a := unren a in
+  let b := unren b in
+  constr:(tPair A B a b)
+| _ => t
+end.
+
+Lemma dred_ren_adj : forall t u ρ, [t⟨ρ⟩ ⇶ u] -> ∑ u', u = u'⟨ρ⟩.
+Proof.
+intros t u ρ Hr.
+remember t⟨ρ⟩ as t' eqn:Ht.
+revert t ρ Ht; induction Hr; intros t₀ ρ Ht.
+all: repeat match goal with H : _ = ?t⟨?ρ⟩ |- _ =>
+  destruct t; cbn in *; try discriminate; [idtac];
+  try injection H; intros; subst
+end.
+all: repeat match goal with H : forall (t : term) (ρ : nat -> nat), _ |- _ =>
+  specialize (H _ _ eq_refl); destruct H; subst
+end.
+all: let t := lazymatch goal with |- ∑ n, ?t = _ => t end in
+     try (let t := unren t in now eexists t).
++ assert (Hrw : forall t u, t⟨upRen_term_term ρ⟩[(u⟨ρ⟩)..] = (t[u..])⟨ρ⟩) by now asimpl.
+  rewrite Hrw; now eexists.
+Qed.
+
+Lemma redalg_ren_inv : forall t u ρ, ren_inj ρ -> [t⟨ρ⟩ ⇶* u⟨ρ⟩] -> [t ⇶* u].
+Proof.
+intros t u ρ Hρ Hr.
+remember t⟨ρ⟩ as t' eqn:Ht.
+remember u⟨ρ⟩ as u' eqn:Hu.
+revert t u ρ Ht Hu Hρ; induction Hr; intros; subst.
++ intros; subst.
+  apply ren_inj_inv in Hu; now subst.
++ unshelve eassert (H := dred_ren_adj _ _ _ _); [..|tea|].
+  destruct H; subst.
+  econstructor; [|eapply IHHr]; eauto.
+  now eapply dred_ren_inv.
 Qed.
 
 (** Derived rules *)
@@ -209,7 +585,9 @@ Proof.
 induction 1.
 + reflexivity.
 + econstructor; [|eassumption].
-  now econstructor.
+  econstructor; [|eassumption].
+  destruct t; try constructor.
+  all: eelim whnf_nored; [eapply whnf_tLambda|eassumption].
 Qed.
 
 Lemma redalg_natElim {P hs hz t t'} : [t ⤳* t'] -> [tNatElim P hs hz t ⤳* tNatElim P hs hz t'].
@@ -217,7 +595,10 @@ Proof.
 induction 1.
 + reflexivity.
 + econstructor; [|eassumption].
-  now econstructor.
+  econstructor; [|eassumption].
+  destruct t; try constructor.
+  - eelim whnf_nored; [eapply whnf_tZero|eassumption].
+  - eelim whnf_nored; [eapply whnf_tSucc|eassumption].
 Qed.
 
 Lemma redalg_natEmpty {P t t'} : [t ⤳* t'] -> [tEmptyElim P t ⤳* tEmptyElim P t'].
@@ -231,20 +612,280 @@ Qed.
 Lemma redalg_fst {t t'} : [t ⤳* t'] -> [tFst t ⤳* tFst t'].
 Proof.
   induction 1; [reflexivity|].
-  econstructor; tea; now constructor.
+  econstructor; tea.
+  constructor; tea.
+  destruct t; try constructor.
+  eelim whnf_nored; [eapply whnf_tPair|eassumption].
 Qed.
 
 Lemma redalg_snd {t t'} : [t ⤳* t'] -> [tSnd t ⤳* tSnd t'].
 Proof.
   induction 1; [reflexivity|].
-  econstructor; tea; now constructor.
+  econstructor; tea.
+  constructor; tea.
+  destruct t; try constructor.
+  eelim whnf_nored; [eapply whnf_tPair|eassumption].
 Qed.
 
 Lemma redalg_idElim {A x P hr y t t'} : [t ⤳* t'] -> [tIdElim A x P hr y t ⤳* tIdElim A x P hr y t'].
 Proof.
   induction 1; [reflexivity|].
-  econstructor; tea; now constructor.
+  econstructor; tea; constructor; [|tea].
+  destruct t; try constructor.
+  eelim whnf_nored; [eapply whnf_tRefl|eassumption].
 Qed.
 
 Lemma redalg_one_step {t t'} : [t ⤳ t'] -> [t ⤳* t'].
 Proof. intros; econstructor;[tea|reflexivity]. Qed.
+
+Lemma dredalg_prod : forall A A₀ B B₀,
+  [A ⇶* A₀] -> dnf A₀ ->
+  [B ⇶* B₀] -> [tProd A B ⇶* tProd A₀ B₀].
+Proof.
+intros A A₀ B B₀ HRA HAnf HRB.
+transitivity (tProd A₀ B).
+- clear - HRA HAnf; induction HRA.
+  * constructor.
+  * econstructor; [|now eauto].
+    now constructor.
+- clear - HAnf HRB; induction HRB.
+  * constructor.
+  * econstructor; [|now eauto].
+    now constructor.
+Qed.
+
+Lemma dredalg_lambda : forall A A₀ t t₀,
+  [A ⇶* A₀] -> dnf A₀ ->
+  [t ⇶* t₀] -> [tLambda A t ⇶* tLambda A₀ t₀].
+Proof.
+intros A A₀ t t₀ HRA HAnf HRt.
+transitivity (tLambda A₀ t).
+- clear - HRA HAnf; induction HRA.
+  * constructor.
+  * econstructor; [|now eauto].
+    now constructor.
+- clear - HAnf HRt; induction HRt.
+  * constructor.
+  * econstructor; [|now eauto].
+    now constructor.
+Qed.
+
+Lemma dredalg_app : forall t t₀ u u₀,
+  whne t ->
+  [t ⇶* t₀] -> dne t₀ -> [u ⇶* u₀] -> [tApp t u ⇶* tApp t₀ u₀].
+Proof.
+intros t t₀ u u₀ Ht HRt Htnf Hru.
+transitivity (tApp t₀ u).
+- clear - HRt Ht Htnf; induction HRt.
+  + constructor.
+  + assert (whne t') by now eapply dred_whne.
+    etransitivity; [|now apply IHHRt].
+    econstructor; [|reflexivity].
+    constructor; [|tea].
+    inversion Ht; subst; eauto.
+- clear - Htnf Hru; induction Hru.
+  + constructor.
+  + econstructor; [|tea].
+    constructor; eauto.
+Qed.
+
+Lemma dredalg_sig : forall A A₀ B B₀,
+  [A ⇶* A₀] -> dnf A₀ ->
+  [B ⇶* B₀] -> [tSig A B ⇶* tSig A₀ B₀].
+Proof.
+intros A A₀ B B₀ HRA HAnf HRB.
+transitivity (tSig A₀ B).
+- clear - HRA HAnf; induction HRA.
+  * constructor.
+  * econstructor; [|now eauto].
+    now constructor.
+- clear - HAnf HRB; induction HRB.
+  * constructor.
+  * econstructor; [|now eauto].
+    now constructor.
+Qed.
+
+Lemma dredalg_pair : forall A A₀ B B₀ a a₀ b b₀,
+  [A ⇶* A₀] -> dnf A₀ -> [B ⇶* B₀] -> dnf B₀ ->
+  [a ⇶* a₀] -> dnf a₀ -> [b ⇶* b₀] -> dnf b₀ ->
+  [tPair A B a b ⇶* tPair A₀ B₀ a₀ b₀].
+Proof.
+intros A A₀ B B₀ a a₀ b b₀ HRA HA HRB HB HRa Ha HRb Hb.
+transitivity (tPair A₀ B a b);
+  [|transitivity (tPair A₀ B₀ a b);
+    [|transitivity (tPair A₀ B₀ a₀ b)]].
+- clear - HRA HA; induction HRA.
+  * constructor.
+  * econstructor; [|now eauto].
+    now constructor.
+- clear - HA HRB; induction HRB.
+  * constructor.
+  * econstructor; [|now eauto].
+    now constructor.
+- clear - HA HB HRa; induction HRa.
+  * constructor.
+  * econstructor; [|now eauto].
+    now constructor.
+- clear - HA HB Ha HRb; induction HRb.
+  * constructor.
+  * econstructor; [|now eauto].
+    now constructor.
+Qed.
+
+Lemma dredalg_fst : forall t t₀,
+  whne t ->
+  [t ⇶* t₀] -> [tFst t ⇶* tFst t₀].
+Proof.
+intros t t₀ Ht HRt.
+induction HRt.
+- constructor.
+- assert (whne t') by now eapply dred_whne.
+  econstructor; [|now eauto].
+  constructor; [|tea].
+  inversion Ht; subst; eauto.
+Qed.
+
+Lemma dredalg_snd : forall t t₀,
+  whne t ->
+  [t ⇶* t₀] -> [tSnd t ⇶* tSnd t₀].
+Proof.
+intros t t₀ Ht HRt.
+induction HRt.
+- constructor.
+- assert (whne t') by now eapply dred_whne.
+  econstructor; [|now eauto].
+  constructor; [|tea].
+  inversion Ht; subst; eauto.
+Qed.
+
+Lemma dredalg_succ : forall n n₀, [n ⇶* n₀] -> [tSucc n ⇶* tSucc n₀].
+Proof.
+intros n n₀ HRn; induction HRn.
+- reflexivity.
+- econstructor; [|tea].
+  now constructor.
+Qed.
+
+Lemma dredalg_natElim : forall P P₀ hz hz₀ hs hs₀ t t₀,
+  whne t -> [t ⇶* t₀] -> dne t₀ ->
+  [P ⇶* P₀] -> dnf P₀ -> [hz ⇶* hz₀] -> dnf hz₀ -> [hs ⇶* hs₀] -> dnf hs₀ ->
+  [tNatElim P hz hs t ⇶* tNatElim P₀ hz₀ hs₀ t₀].
+Proof.
+intros P P₀ hz hz₀ hs hs₀ t t₀ Ht HRt Hne HRP HP HRhz Hhz HRhs Hhs.
+transitivity (tNatElim P hz hs t₀);
+  [|transitivity (tNatElim P₀ hz hs t₀);
+    [|transitivity (tNatElim P₀ hz₀ hs t₀)]].
+- clear - HRt Ht Hne; induction HRt.
+  + constructor.
+  + assert (whne t') by now eapply dred_whne.
+    econstructor; [|now eauto].
+    constructor; [|tea].
+    inversion Ht; subst; eauto.
+- clear - HRP HP Hne; induction HRP.
+  + constructor.
+  + econstructor; [|now eauto].
+    constructor; eauto.
+- clear - HRhz Hne HP; induction HRhz.
+  + constructor.
+  + econstructor; [|now eauto].
+    constructor; eauto.
+- clear - HRhs Hne HP Hhz; induction HRhs.
+  + constructor.
+  + econstructor; [|now eauto].
+    constructor; eauto.
+Qed.
+
+Lemma dredalg_emptyElim : forall P P₀ t t₀,
+  whne t -> [t ⇶* t₀] -> dne t₀ ->
+  [P ⇶* P₀] -> dnf P₀ ->
+  [tEmptyElim P t ⇶* tEmptyElim P₀ t₀].
+Proof.
+intros P P₀ t t₀ Ht HRt Hne HRP HP.
+transitivity (tEmptyElim P t₀).
+- clear - HRt Ht Hne; induction HRt.
+  + constructor.
+  + assert (whne t') by now eapply dred_whne.
+    econstructor; [|now eauto].
+    constructor; [|tea].
+    inversion Ht; subst; eauto.
+- clear - HRP HP Hne; induction HRP.
+  + constructor.
+  + econstructor; [|now eauto].
+    constructor; eauto.
+Qed.
+
+Lemma dredalg_id : forall A A₀ t t₀ u u₀,
+  [A ⇶* A₀] -> dnf A₀ -> [t ⇶* t₀] -> dnf t₀ -> [u ⇶* u₀] -> dnf u₀ ->
+  [tId A t u ⇶* tId A₀ t₀ u₀].
+Proof.
+intros A A₀ t t₀ u u₀ HRA HAnf HRt Htnf HRu Hunf.
+transitivity (tId A₀ t u); [|transitivity (tId A₀ t₀ u)]; [| |].
+- clear - HRA HAnf; induction HRA.
+  * constructor.
+  * econstructor; [|now eauto].
+    now constructor.
+- induction HRt.
+  * constructor.
+  * econstructor; [|now eauto].
+    now constructor.
+- induction HRu.
+  * constructor.
+  * econstructor; [|now eauto].
+    now constructor.
+Qed.
+
+Lemma dredalg_refl : forall A A₀ x x₀,
+  [A ⇶* A₀] -> dnf A₀ -> [x ⇶* x₀] ->
+  [tRefl A x ⇶* tRefl A₀ x₀].
+Proof.
+intros A A₀ x x₀ HRA HAnf HRx.
+transitivity (tRefl A₀ x).
+- clear - HRA HAnf; induction HRA.
+  * constructor.
+  * econstructor; [|now eauto].
+    now constructor.
+- clear - HAnf HRx; induction HRx.
+  * constructor.
+  * econstructor; [|now eauto].
+    now constructor.
+Qed.
+
+Lemma dredalg_idElim : forall A A₀ x x₀ P P₀ hr hr₀ y y₀ t t₀,
+  whne t -> [t ⇶* t₀] -> dne t₀ ->
+  [A ⇶* A₀] -> dnf A₀ -> [x ⇶* x₀] -> dnf x₀ ->
+  [P ⇶* P₀] -> dnf P₀ -> [hr ⇶* hr₀] -> dnf hr₀ -> [y ⇶* y₀] -> dnf y₀ ->
+  [tIdElim A x P hr y t ⇶* tIdElim A₀ x₀ P₀ hr₀ y₀ t₀].
+Proof.
+intros A A₀ x x₀ P P₀ hr hr₀ y y₀ t t₀ Ht HRt Hne HRA HA HRx Hx HRP HP HRhr Hhr HRy Hy.
+transitivity (tIdElim A x P hr y t₀);
+  [|transitivity (tIdElim A₀ x P hr y t₀);
+    [|transitivity (tIdElim A₀ x₀ P hr y t₀);
+      [|transitivity (tIdElim A₀ x₀ P₀ hr y t₀);
+        [|transitivity (tIdElim A₀ x₀ P₀ hr₀ y t₀)]]]].
+- clear - HRt Ht Hne; induction HRt.
+  + constructor.
+  + assert (whne t') by now eapply dred_whne.
+    econstructor; [|now eauto].
+    constructor; [|tea].
+    inversion Ht; subst; eauto.
+- clear - HRA HA Hne; induction HRA.
+  + constructor.
+  + econstructor; [|now eauto].
+    constructor; eauto.
+- clear - HRx Hne HA; induction HRx.
+  + constructor.
+  + econstructor; [|now eauto].
+    constructor; eauto.
+- clear - HRP Hne HA Hx; induction HRP.
+  + constructor.
+  + econstructor; [|now eauto].
+    constructor; eauto.
+- clear - HRhr Hne HA Hx HP; induction HRhr.
+  + constructor.
+  + econstructor; [|now eauto].
+    constructor; eauto.
+- clear - HRy Hne HA Hx HP Hhr; induction HRy.
+  + constructor.
+  + econstructor; [|now eauto].
+    constructor; eauto.
+Qed.
